# Quiz #2
David McNeary
COMP 256
3/1/2022

## Problem 1:
a.

$$
\sum_{j=12}^{15} 52^{3j-7} \\
= 52^{3(12)-7} + 52^{3(13)-7} + 52^{3(14-7} + 52^{3(15)-7} \\
= 52^{36-7} + 52^{39-7} + 52^{42-7} + 52^{45-7} \\
= 52^{29} + 52^{32} + 52^{35} + 52^{38}
$$

b.

$$
\sum_{i=25}^{27} \frac{i^2}{(i - 29)} \\
= \frac{25^2}{(25-29)} + \frac{26^2}{(26-29)} + \frac{27^2}{(27-29)} \\
= \frac{25^2}{(-4)} + \frac{26^2}{(-3)} + \frac{27^2}{(-2)}
$$

c.

$$
\sum^6_{i=4}\sum^3_{j=1}i(3j-2j)^{j-1} \\
= \sum^6_{i=4}i\sum^3_{j=1}(3j-2j)^{j-1} \\
= \sum^6_{i=4}i[(3(1) - 2(1))^{1-1} + (3(2) - 2(2))^{2-1} + (3(3) - 2(3))^{3-1}] \\
= \sum^6_{i=4}i[(3 - 2)^0 + (6 - 4)^1 + (9 - 6)^2] \\
=\sum^6_{i=4}i(1^0 + 2^1 + 3^2) \\
=\sum^6_{i=4}i(1 + 2 + 9) \\
=\sum^6_{i=4}i(12) \\
=12\sum^6_{i=4}i \\
=12(4 + 5 + 6) \\
=12(15) \\
= 180
$$

d.

$$
\sum^7_{k=1}\sum^{39}_{j=0}4kj \\
= \sum^7_{k=1}4k\sum^{39}_{j=0}j \\
= 4\sum^7_{k=1}k\sum^{39}_{j=0}j \\
= 4\sum^7_{k=1}k\frac{39(39+1)}{2} \\
= (4)\frac{39(39+1)}{2}\sum^7_{k=1}k \\
= (4)\frac{39(39+1)}{2}\frac{7(7+1)}{2} \\
= (2)(39)(40)(7)(8) \\
= 174720
$$

e.

$$
\sum^4_{j=1}\sum^{j}_{i=0}20i \\
= \sum^4_{j=1}20\sum^{j}_{i=0}i \\
= \sum^4_{j=1}20\frac{j(j+1)}{2} \\
= \frac{20}{2}\sum^4_{j=1}j^2 + j \\
= 10(\sum^4_{j=1}j^2 + \sum^4_{j=1}j) \\
\space \\
= 10[\frac{4(4+1)[2(4)+1]}{2} + \frac{4(4+1)}{2}] \\
\space \\
= 10[\frac{4(5)(8+1) + 4(5)}{2}] \\
\space \\
= 5[4(5)(9) + 4(5)] \\
= 5[180 + 20] \\
= 5[200] \\
= 1000
$$

f.
$$
\sum_{k\in S}(5 + \sum_{j \in S}j), S = \{3, 7, 6, 14, 15\} \\
= (5 + \sum_{j \in S}j)\sum_{k\in S}1 \\
= [5 + (3 + 7 + 6 + 14 + 15)]\sum_{k\in S}1 \\
= (5 + 45)\sum^5_{k = 0}1 \\
= 50(5) \\
= 250
$$

g. 

$$
\sum^{119}_{j = 51}j - \sum^{1274}_{i = 0}i \\
= (\sum^{119}_{j = 0}j - \sum^{50}_{j = 0}j) - \sum^{1274}_{i = 0}i \\
\space \\
= \frac{119(119+1)}{2} - \frac{50(50+1)}{2} - \frac{1274(1274+1)}{2} \\
\space \\
= \frac{119(120)}{2} - \frac{50(51)}{2} - \frac{1274(1275)}{2} \\
\space \\
= \frac{14280}{2} - \frac{2550}{2} - \frac{1624350}{2} \\
\space \\
= \frac{(-1612620)}{2} \\
\space \\
= (-806310)
$$

## Problem 2:
a.
```
for (k= 0; k ≤ 2n 3+5n+7; k++){
    print “Hello”;}
for (j = 0; j ≤ 7n 3+13; j++){
    print “Hello”;}
for (i = 1; i ≤ (3n-8)(n+2); i++){
    print “Hello”;}
```

$$
\sum_{k =0}^{2n^3 + 5n + 7 + 1}1 + \sum_{j =0}^{7n^3 + 13 + 1}1 + \sum_{i =0}^{(3n - 8)(n+2)}1 \\
= 2n^3 + 5n + 8 + 7n^3 + 14 + (3n - 8)(n+2) \\
= 9n^3 + 5n + 22 + (3n^2 + 6n - 8n - 16) \\
= 9n^3 + 3n^2 + 5n - 2n + 22 - 16 \\
= 9n^3 + 3n^2 + 3n + 6
$$

b.
```
k = 0;
while (k ≤ n){
    for (i = 0; i ≤ k-1; i++){
        print “hello”;
        print “hello”;
        print “hello”;}
    k = 5k;
    print “hello”;
    print “hello”;}
```

$$
\sum_{k=0}^{\log_5 n}2\sum_{i = 0}^{k - 1}3 \\
= (2)(3)\sum_{k=0}^{\log_5 n}1\sum_{i = 0}^{k - 1}1 \\
= 6(\sum_{k=0}^{\log_5 n}k - 1) \\
= 6(\sum_{k=0}^{\log_5 n}k - \sum_{k=0}^{\log_5 n}1) \\
\space \\
= 6(\frac{\log_5 n(\log_5 n + 1)}{2} - \log_5 n) \\
= 6(\frac{(\log_5 n)^2 + \log_5 n)}{2} - \log_5 n) \\
= 3(\log_5 n)^2 + 3\log_5 n - \log_5 n \\
= 3(\log_5 n)^2 + 2\log_5 n
$$

c.
```
for (i = 1; i ≤ 7n+5; i++){
    for (j = 0; j ≤ i-1; j++){
        for (k = 0; k ≤ 3; k++){
            print “Hello”;}}}
```

$$
\sum_{i = 1}^{7n+5}\sum_{j = 0}^{i - 1 + 1}\sum_{k = 0}^{3 + 1} 1 \\
= \sum_{i = 1}^{7n+5}\sum_{j = 0}^{i - 1 + 1}4 \\
= \sum_{i = 1}^{7n+5}4\sum_{j = 0}^{i - 1 + 1}1 \\
= \sum_{i = 1}^{7n+5}4i \\
= 4\sum_{i = 1}^{7n+5}i \\
\space \\
= 4\frac{(7n+5)(7n + 5 + 1)}{2} \\
\space \\
= 2(7n+5)(7n + 6) \\
= 2(49n^2 + 42n + 35n + 30) \\
= 98n^2 + 77n + 60
$$

d.
```
for (i = 0; i ≤ n; i = i + 9){
    for (k = 0; k ≤ n; k++){
        print “Hello”;}
    print “Hello”;
    print “Hello”;
    for (j = 1; j ≤ n; j++){
        print “Hello”;
        print “Hello”;
        print “Hello”;}}
```

$$
\sum_{i = 0}^{n/9}2(\sum_{k = 0}^n1 + \sum_{j = 1}^n3) \\
= 2\sum_{i = 0}^{n/9}1(n + 3n) \\
= 2(n + 3n)\sum_{i = 0}^{n/9}1 \\
= (2n + 6n)(n/9) \\
= \frac{8n^2}{9}
$$

e.
```
for (j = 0; j ≤ 7n-3; j++){
    for (i = 1, i ≤ n; i = 5i){
        print “Hello”;
        print “Hello”;
        print “Hello”;
        for (k = 0; k ≤ log! 16; k++){
            print “Hello”;
            print “Hello”;}}}
```

$$
\sum^{7n - 3 + 1}_{j = 0}\sum_{i = 1}^{\log_5 n}3\sum_{k = 0}^{\log_2 16}2 \\
= \sum^{7n - 3 + 1}_{j = 0}3\sum_{i = 1}^{\log_5 n}1(2)\sum_{k = 0}^{4}1 \\
= \sum^{7n - 3 + 1}_{j = 0}3\sum_{i = 1}^{\log_5 n}(2)(4) \\
= \sum^{7n - 3 + 1}_{j = 0}3(8)\sum_{i = 1}^{\log_5 n}1 \\
= 24\sum^{7n - 2}_{j = 0}\sum_{i = 1}^{\log_5 n}1 \\
= 24\sum^{7n - 2}_{j = 0}\log_5 n \\
= 24\log_5 n\sum^{7n - 2}_{j = 0}1 \\
= 24(\log_5 n)(7n - 2) \\
$$

f.
```
for (k = 1; k ≤ 7n3; k = 4k){
    print “Hello”;
    for (j = 1; j ≤ n; j = j + 4){
        print “Hello”;}
    print “Hello”;}
```

$$
\sum^{\log_47n^3}_{k = 1}2\sum_{j = 1}^{n/4}1 \\
= 2\sum^{\log_47n^3}_{k = 1}n/4 \\
= (n/2)\log_4 7n^3 \\
$$