# Proofs
February 22, 2022

Proofs are all about writing clear and thorough logical steps towards a solution to a problem. Various methods of proofs include direct proofs, contradiction, contrapositive proofs, proof by cases, and proof by induction. The first three use similar methods in their techniques, but induction methodology is a bit odd in this collection.

Most often in this class, we will be proving conditional statements, in the form of "if p, then q."

## Direct Proofs
For a statement $p\rightarrow q$, we typically assume that $p$ is true, then try to prove $q$.

Let's try to prove the following: the sum of an even number $m$ and an odd number $n$ is odd.

$$
\text{Prove: }m \cap n \rightarrow (m + n)\mod 2 \gt 0  \\
\space \\
\text{Let } m = \\{x|k\in\mathbb{Z} \cap x = 2k\\}, \\
n = \\{y|t\in\mathbb{Z} \cap y = 2t + 1\\} \\
\space \\
x + y = 2k + 2t + 1 \\
= 2(k + t) + 1 \\
\therefore x + y\rightarrow m \cap n
$$

## Contrapositive
Contrapositive takes a similar approach to direct proofs, but in an inverted manner. Contrapositives seek to prove $p \rightarrow q$ by instead proving $\lnot q \rightarrow \lnot p$.

Let's proof that if $3n + 2$ is odd, then $n$ is odd:

$$
\text{Let }n = \\{n|k\in\mathbb{Z} \cap n = 2k\\} \\
\space \\
3n + 2 = 3(2n) + 2 = 2(3n + 1) \\
n = 2k \cap 3k + 1 \in \mathbb{Z} \rightarrow (3n + 2)\mod 2 = 0 \\
\therefore \lnot (3n + 2)\mod 2 = 0 \rightarrow \lnot (n = 2k)
$$

In other words, letting $p$ represent "$n$ is even" and $q$ represent "$3n + 2$ is even," then $\lnot q \rightarrow \lnot p$. So, if $3n + 2$ is odd, then $n$ is odd.

Another example:

$$
\text{Prove: }n=ab \rightarrow (a \le \sqrt{n}) \cup (b \le \sqrt{n}) \\
\space \\
\lnot q = \lnot [(a \le \sqrt{n}) \cup (b \le \sqrt{n})] \\
= \lnot(a \le \sqrt{n}) \cap \lnot(b \le \sqrt{n}) \\
=(a \gt \sqrt{n}) \cap (b\gt\sqrt{n}) \\
\space \\
\lnot p = n \not = ab \\
\space \\
(a \gt \sqrt{n}) \cap (b\gt\sqrt{n}) \rightarrow ab \gt n \\
\lnot [(a \le \sqrt{n}) \cup (b \le \sqrt{n})] \rightarrow  ab \not= n \\
\therefore n=ab \rightarrow (a \le \sqrt{n}) \cup (b \le \sqrt{n})
$$

## Contradiction
Contradiction utilizes the equivalence that $p$ is true if and only if when if $p$ is not true, then $F_0$ is true, where $F_0$ is an universally false statement:

$$
p \iff \lnot p \rightarrow F_0
$$

Let's re-visit a question above: if $3n + 2$ is odd, then $n$ is odd:

$$
n \mod 2 = 0 \rightarrow n=2k, \\{k|k\in\mathbb{Z}\\} \\
\space \\
3n + 2 = 3(2k) + 2
= 2(3k + 1) \\
2k \not = 3k + 1 \\
\therefore \lnot (n=2k) \rightarrow n\mod 2 \not = 0
$$