# Proof by Induction
March 3, 2022

## Induction Algorithm
Starting with a base case (1), an inductive hypothesis is made and proved via math. The base case is the simplest, or smallest, possible value. From the base case, an inductive hypothesis (2) for a general value $k$ may be assumed. Proving that $k + 1$ is also true by using the hypothesis (3) completes the proof.

Algorithm:
1. Base case
2. Inductive hypothesis
3. Inductive proof

---

Suppose we want to prove the following:

$$
\sum_{i = 1}^n i(i + 1) = \frac{n(n+1)(n+2)}{3}, \forall n \ge 1
$$

The base case would substitute the value $1$ for all $n$:

$$
\sum_{i = 1}^1 i(i + 1) = \frac{1(1+1)(1+2)}{3} \\
1(1 + 1) = \frac{1(2)(3)}{3} \\
1(2) = \frac{6}{3} \\ \space \\
2 = 2
$$

Then, we assume that a hypothesis is true, substituting in $k$:

$$
\sum_{i = 1}^k i(i + 1) = \frac{k(k+1)(k+2)}{3}, \forall k\ge 1 \\
$$

We can then attempt to prove the general case $k + 1$:

$$
\sum_{i = 1}^{k + 1} i(i + 1) \overset{?}{=} \frac{(k+1)(k+1+1)(k+1+2)}{3} \\
\sum_{i = 1}^{k + 1} i(i + 1) = \sum_{i = 1}^{k} i(i + 1) + (k + 1)(k + 1 + 1) \\
= \frac{k(k+1)(k+2)}{3} + (k + 1)(k + 2) \\
= (k + 1)(k + 2)(\frac{k}{3} + 1) \\
\space \\
= \frac{3}{3}(k + 1)(k + 2)(\frac{k}{3} + 1) \\
\space \\
= \frac{(k + 1)(k + 2)(\frac{k}{3} + 1)(3)}{3} \\
\space \\
= \frac{(k+1)(k+2)(k+3)}{3} \\
\space \\
= \frac{(k+1)(k+1+1)(k+1+2)}{3}\\
\space \\
\therefore \sum_{i = 1}^{k + 1} i(i + 1) = \frac{(k+1)(k+1+1)(k+1+2)}{3} 
$$

---

More practice:

$$
\sum^n_{i = 0} 2^i = 2^{n + 1} - 1, \forall n \ge 0
$$

Base case:

$$
n = 0 \rightarrow P(0) \\
\sum^0_{i = 0} 2^i = 2^{0 + 1} - 1 \\
2^0 = 2 - 1 \\
\therefore 1 = 1
$$

Hypothesis: Assume $P(k)$ is true for $\forall k \ge 0$:

$$
\sum^k_{i = 0} 2^i = 2^{k + 1} - 1
$$

Now prove for a general $P(k + 1)$:

$$
\sum^{k + 1}_{i = 0} 2^i \overset{?}{=} 2^{(k + 1) + 1} - 1 \\
\sum^{k + 1}_{i = 0} 2^i = \sum^{k}_{i = 0} 2^i + 2^{k + 1} \\
= 2^{k + 1} - 1 + 2^{k + 1} \\
= (2)2^{k + 1} - 1 \\
= (2^1)(2^{k + 1}) - 1 \\
= 2^{k + 2} - 1 \\
\space \\
\therefore \sum^{k + 1}_{i = 0} 2^i= 2^{k + 2} - 1
$$

---

## Divisibility Proofs
When attempting whether a number is divisible by another number, we are saying that there is an integer quotient with no remainder.

Lets try to prove the following: $6^n + 4$ is divisible by $5$ for $\forall n \ge 0$:

Base case:

$$
n = 0: P(0) = 6^0 + 4 \text{ is divisible by } 5 \\
6^0 + 4 = 1 + 4 = 5 \rightarrow \\
\frac{5}{5} = 1 \\
\space \\
\therefore P(0) \text { is true}
$$

Assume $P(k)$ is true for $\forall k \ge 0$:

$$
P(k) = 6^k + 4 \text{ is divisible by } 5
$$

Prove for $P(k + 1)$:

$$
P(k) = 6^{k+1} + 4 \text{ is divisible by } 5? \\
\space \\
6^{k+1} + 4 = (6^1)(6^k) + 4 \\
= (6)6^k + (6)4 + 4 - (6)4 \\
= 6(6^k + 4) + 4(1-6) \\
= 6(6^k + 4) - 20 \\
$$

Since $6^k + 4$ is a multiple of $5$ by our hypothesis, and $20$ is divisible by $5$, we've completed the proof:

$$
\therefore 6^{k+1} + 4 \text{ is divisible by } 5 \text{ by hyp.}
$$

## Inequalities
Lets try induction with an inequality:
Prove $2^{n+1} \gt n^2, \forall n \ge 3$

Base case: $P(3)$

$$
n = 3 \rightarrow 2^{3+1} \gt 3^2 \\
2^4 \gt 9 \\
16 \gt 9
$$

Hypothesis: Assume P(k) is true:

$$
2^{k + 1} \gt k^2, \forall k \ge 3
$$

Proof of $P(k + 1), \forall k \ge 3$:

$$
2^{(k + 1) + 1} \gt (k + 1)^2 \\
2^{k + 2} \gt k^2 + 2k + 1 \\
(2)2^{k+1} \gt k^2 + 2k + 1 \\
\space \\
\forall k \ge 3: 
2^{k + 1} \overset{\text{by hyp}}{\gt} k^2 \rightarrow (2)2^{k + 1} \gt 2k^2 \\
\space \\
\forall k \ge 3: 
2k^2 \overset{?}{\gt}k^2 + 2k + 1 \\
k^2 \gt 2k + 1 \\
k^2 - 2k - 1 \gt 0 \\
\therefore (2)2^{k+1} \gt 2k^2 \gt k^2 + 2k + 1 \rightarrow 2^{(k + 1) + 1} \gt (k + 1)^2
$$